proof/invariant-abstract/X64/ArchCrunchSetup_AI.thy
@@ -1,0 +1,23 @@
+(*
+ * Copyright 2014, General Dynamics C4 Systems
+ *
+ * This software may be distributed and modified according to the terms of
+ * the GNU General Public License version 2. Note that NO WARRANTY is provided.
+ * See "LICENSE_GPLv2.txt" for details.
+ *
+ * @TAG(GD_GPL)
+ *)
+
+theory ArchCrunchSetup_AI
+imports
+  "../../../spec/abstract/Syscall_A"
+  "../../../lib/Crunch"
+begin
+context Arch begin global_naming X64
+
+
+crunch_ignore (add: debugPrint clearMemory invalidateTLB initL2Cache)
+
+end
+
+end
