proof/invariant-abstract/X64/ArchKHeap_AI.thy
@@ -1,0 +1,587 @@
+(*
+ * Copyright 2014, General Dynamics C4 Systems
+ *
+ * This software may be distributed and modified according to the terms of
+ * the GNU General Public License version 2. Note that NO WARRANTY is provided.
+ * See "LICENSE_GPLv2.txt" for details.
+ *
+ * @TAG(GD_GPL)
+ *)
+
+theory ArchKHeap_AI
+imports "../KHeapPre_AI"
+begin
+
+context Arch begin global_naming ARM
+
+
+sublocale
+  empty_table: arch_only_obj_pred "empty_table S" for S
+  by (unfold_locales, simp add: empty_table_def del: arch_obj_fun_lift_expand)
+
+sublocale
+  vs_refs: arch_only_obj_pred "\<lambda>ko. x \<in> vs_refs ko"
+  by (unfold_locales, simp add: vs_refs_def del: vs_refs_arch_def)
+
+sublocale
+  vs_refs_pages: arch_only_obj_pred "\<lambda>ko. x \<in> vs_refs_pages ko"
+  by (unfold_locales, simp add: vs_refs_pages_def del: vs_refs_pages_arch_def)
+
+lemma pspace_in_kernel_window_atyp_lift_strong:
+  assumes atyp_inv: "\<And>P p T. \<lbrace> \<lambda>s. P (typ_at T p s) \<rbrace> f \<lbrace> \<lambda>rv s. P (typ_at T p s) \<rbrace>"
+  assumes arch_inv: "\<And>P. \<lbrace>\<lambda>s. P (arm_kernel_vspace (arch_state s))\<rbrace> f \<lbrace>\<lambda>r s. P (arm_kernel_vspace (arch_state s))\<rbrace>"
+  shows      "\<lbrace>\<lambda>s. pspace_in_kernel_window s\<rbrace> f \<lbrace>\<lambda>rv s. pspace_in_kernel_window s\<rbrace>"
+  apply (simp add: pspace_in_kernel_window_def)
+  apply (rule hoare_lift_Pf[where f="\<lambda>s. arm_kernel_vspace (arch_state s)", OF _ arch_inv])
+   apply (rule hoare_vcg_all_lift)
+   apply (simp add: obj_bits_T)
+   apply (simp add: valid_def)
+  apply clarsimp
+  subgoal for _ x s _ _ ko
+  apply (cases "kheap s x")
+  apply (frule use_valid[OF _ atyp_inv, where P1= "\<lambda>x. \<not> x" and T1="a_type ko" and p1=x];
+          simp add: obj_at_def a_type_def)
+
+   subgoal for ko'
+   apply (drule spec[of _ ko'])
+   apply (simp add: obj_bits_T)
+   apply (frule use_valid[OF _ atyp_inv, where P1= "\<lambda>x. x" and T1="a_type ko'" and p1=x])
+   by (simp add: obj_at_def a_type_def)+
+ done
+ done
+
+lemma pspace_in_kernel_window_atyp_lift:
+  assumes atyp_inv: "\<And>P p T. \<lbrace>\<lambda>s. P (typ_at T p s)\<rbrace> f \<lbrace>\<lambda>rv s. P (typ_at T p s)\<rbrace>"
+  assumes arch_inv: "\<And>P. \<lbrace>\<lambda>s. P (arch_state s)\<rbrace> f \<lbrace>\<lambda>r s. P (arch_state s)\<rbrace>"
+  shows      "\<lbrace>\<lambda>s. pspace_in_kernel_window s\<rbrace> f \<lbrace>\<lambda>rv s. pspace_in_kernel_window s\<rbrace>"
+  by (rule pspace_in_kernel_window_atyp_lift_strong[OF atyp_inv arch_inv])
+
+lemma cap_refs_in_kernel_window_arch_update[simp]:
+  "arm_kernel_vspace (f (arch_state s)) = arm_kernel_vspace (arch_state s)
+     \<Longrightarrow> cap_refs_in_kernel_window (arch_state_update f s) = cap_refs_in_kernel_window s"
+  by (simp add: cap_refs_in_kernel_window_def)
+
+lemma
+  ex_ko_at_def2: 
+  "(\<exists>ko. ko_at ko p s \<and> P ko) = (obj_at P p s)"
+  by (simp add: obj_at_def)
+
+lemma vs_lookup_arch_obj_at_lift:
+  assumes obj_at: "\<And>P P' p. arch_obj_pred P' \<Longrightarrow>
+                             \<lbrace>\<lambda>s. P (obj_at P' p s)\<rbrace> f \<lbrace>\<lambda>r s. P (obj_at P' p s)\<rbrace>"
+  assumes arch_state: "\<And>P. \<lbrace>\<lambda>s. P (arch_state s)\<rbrace> f \<lbrace>\<lambda>r s. P (arch_state s)\<rbrace>"
+  shows "\<lbrace>\<lambda>s. P (vs_lookup s)\<rbrace> f \<lbrace>\<lambda>rv s. P (vs_lookup s)\<rbrace>"
+  apply (simp add: vs_lookup_def vs_lookup1_def)
+  apply (simp add: ex_ko_at_def2)
+  apply (rule hoare_lift_Pf[where f="arch_state", OF _ arch_state])
+  apply (rule hoare_lift_Pf[where f="\<lambda>s rs p rs' p'. obj_at (P' p rs rs' p') p s" for P'])
+   apply (rule hoare_vcg_prop)
+  apply (clarsimp simp add: valid_def)
+  apply (erule_tac P=P in rsubst)
+  apply (rule ext)+
+  apply (erule use_valid, rule obj_at, simp)
+  by (auto simp: vs_refs.arch_only
+           intro!: arch_obj_pred_fI[where f=Ex])
+
+lemma vs_lookup_pages_arch_obj_at_lift:
+  assumes obj_at: "\<And>P P' p. arch_obj_pred P' \<Longrightarrow>
+                            \<lbrace>\<lambda>s. P (obj_at P' p s)\<rbrace> f \<lbrace>\<lambda>r s. P (obj_at P' p s)\<rbrace>"
+  assumes arch_state: "\<And>P. \<lbrace>\<lambda>s. P (arch_state s)\<rbrace> f \<lbrace>\<lambda>r s. P (arch_state s)\<rbrace>"
+  shows "\<lbrace>\<lambda>s. P (vs_lookup_pages s)\<rbrace> f \<lbrace>\<lambda>rv s. P (vs_lookup_pages s)\<rbrace>"
+  apply (simp add: vs_lookup_pages_def vs_lookup_pages1_def)
+  apply (simp add: ex_ko_at_def2)
+  apply (rule hoare_lift_Pf[where f="arch_state", OF _ arch_state])
+  apply (rule hoare_lift_Pf[where f="\<lambda>s rs p rs' p'. obj_at (P' p rs rs' p') p s" for P'])
+   apply (rule hoare_vcg_prop)
+  apply (clarsimp simp add: valid_def)
+  apply (erule_tac P=P in rsubst)
+  apply (rule ext)+
+  apply (erule use_valid, rule obj_at, simp)
+  by (auto simp: vs_refs_pages.arch_only
+           intro!: arch_obj_pred_fI[where f=Ex])
+
+lemma valid_arch_objs_lift_weak:
+  assumes obj_at: "\<And>P P' p. arch_obj_pred P' \<Longrightarrow>
+                             \<lbrace>\<lambda>s. P (obj_at P' p s)\<rbrace> f \<lbrace>\<lambda>r s. P (obj_at P' p s)\<rbrace>"
+  assumes arch_state: "\<And>P. \<lbrace>\<lambda>s. P (arch_state s)\<rbrace> f \<lbrace>\<lambda>r s. P (arch_state s)\<rbrace>"
+  shows "\<lbrace>valid_arch_objs\<rbrace> f \<lbrace>\<lambda>_. valid_arch_objs\<rbrace>"
+  apply (rule valid_arch_objs_lift)
+    apply (rule vs_lookup_arch_obj_at_lift)
+     apply (rule obj_at arch_state; simp)+
+  done
+
+lemma set_object_neg_lookup:
+  "\<lbrace>\<lambda>s. \<not> (\<exists>rs. (rs \<rhd> p') s) \<and> obj_at (\<lambda>ko'. vs_refs ko \<subseteq> vs_refs ko') p s \<rbrace> 
+  set_object p ko
+  \<lbrace>\<lambda>_ s. \<not> (\<exists>rs. (rs \<rhd> p') s)\<rbrace>"
+  apply (simp add: set_object_def)
+  apply wp
+  apply clarsimp
+  apply (erule_tac x=rs in allE)
+  apply (erule notE)
+  apply (erule vs_lookup_stateI)
+   apply (clarsimp simp: obj_at_def split: split_if_asm)
+  apply simp
+  done
+
+
+lemma set_object_vs_lookup:
+  "\<lbrace>\<lambda>s. obj_at (\<lambda>ko'. vs_refs ko = vs_refs ko') p s \<and> P (vs_lookup s) \<rbrace> 
+  set_object p ko
+  \<lbrace>\<lambda>_ s. P (vs_lookup s)\<rbrace>"
+  apply (simp add: set_object_def)
+  apply wp
+  apply clarsimp
+  apply (erule rsubst [where P=P])
+  apply (rule order_antisym)
+   apply (rule vs_lookup_sub)
+    apply (clarsimp simp: obj_at_def)
+   apply simp
+  apply (rule vs_lookup_sub)
+   apply (clarsimp simp: obj_at_def split: split_if_asm)
+  apply simp
+  done
+
+
+lemma set_object_pt_not_vs_lookup_pages:
+  "\<lbrace>\<lambda>s. \<not>(ref \<unrhd> p') s
+    \<and> ((\<exists>\<unrhd>p) s \<longrightarrow> (\<forall>x. case pte_ref_pages (pt x) of
+              Some ptr \<Rightarrow> 
+                obj_at (\<lambda>ko. vs_refs_pages ko = {}) ptr s \<and>
+                ptr \<noteq> p'
+            | None \<Rightarrow> True))\<rbrace>
+   set_object p (ArchObj (PageTable pt))
+   \<lbrace>\<lambda>_ s. \<not>(ref \<unrhd> p') s\<rbrace>"
+  apply (simp add: set_object_def)
+  apply wp
+  apply (clarsimp simp: obj_at_def)
+   apply (case_tac "(\<exists>\<unrhd>p) s")
+   apply (erule notE)
+   apply clarsimp
+   apply (subst (asm) vs_lookup_pages_def)
+   apply clarsimp
+   apply (erule vs_lookup_pagesI)
+   apply (erule converse_rtrancl_induct)
+    apply simp
+   apply (drule vs_lookup_pages1D)
+   apply (clarsimp simp: obj_at_def split:split_if_asm)
+   apply (case_tac "pa=p")
+    apply (clarsimp simp: vs_refs_pages_def graph_of_def)
+    apply (erule_tac x=ab in allE)
+    apply (drule_tac R="vs_lookup_pages1 s" in rtranclD)
+    apply clarsimp
+    apply (drule tranclD)
+    apply clarsimp
+    apply (drule vs_lookup_pages1D)
+    apply (clarsimp simp: obj_at_def vs_refs_pages_def)
+   apply clarsimp
+   apply (erule rtrancl_trans[OF r_into_rtrancl, rotated])
+   apply (clarsimp simp: vs_lookup_pages1_def obj_at_def)
+  apply clarsimp
+  apply (erule notE)
+  apply (subst (asm) vs_lookup_pages_def)
+  apply clarsimp
+  apply (rule vs_lookup_pagesI, assumption)
+  apply (erule rtrancl_induct)
+   apply simp
+  apply (drule vs_lookup_pages1D)
+  apply (clarsimp simp: obj_at_def split:split_if_asm)
+  apply (case_tac "pa=p")
+   apply (clarsimp simp: vs_refs_pages_def graph_of_def)
+   apply (erule_tac x=rs in allE)
+   apply (clarsimp simp: vs_lookup_pages_def)
+   apply (drule(1) ImageI, erule (1) notE)
+  apply clarsimp
+  apply (erule rtrancl_trans[OF _ r_into_rtrancl])
+  apply (clarsimp simp: vs_lookup_pages1_def obj_at_def)
+  done
+
+
+lemma set_object_vs_lookup_pages:
+  "\<lbrace>\<lambda>s. obj_at (\<lambda>ko'. vs_refs_pages ko = vs_refs_pages ko') p s \<and> P (vs_lookup_pages s) \<rbrace> 
+  set_object p ko
+  \<lbrace>\<lambda>_ s. P (vs_lookup_pages s)\<rbrace>"
+  apply (simp add: set_object_def)
+  apply wp
+  apply clarsimp
+  apply (erule rsubst [where P=P])
+  apply (rule order_antisym)
+   apply (rule vs_lookup_pages_sub)
+    apply (clarsimp simp: obj_at_def)
+   apply simp
+  apply (rule vs_lookup_pages_sub)
+   apply (clarsimp simp: obj_at_def split: split_if_asm)
+  apply simp
+  done
+
+
+lemma set_object_atyp_at:
+  "\<lbrace>\<lambda>s. typ_at (AArch (aa_type ako)) p s \<and> P (typ_at (AArch T) p' s)\<rbrace> 
+    set_object p (ArchObj ako)
+   \<lbrace>\<lambda>rv s. P (typ_at (AArch T) p' s)\<rbrace>"
+  apply (simp add: set_object_def)
+  apply wp
+  apply clarsimp
+  apply (erule rsubst [where P=P])
+  apply (clarsimp simp: obj_at_def a_type_aa_type)
+  done
+
+lemma set_object_arch_objs:
+  "\<lbrace>valid_arch_objs and typ_at (a_type ko) p and 
+    obj_at (\<lambda>ko'. vs_refs ko \<subseteq> vs_refs ko') p  and
+    (\<lambda>s. case ko of ArchObj ao \<Rightarrow>
+             (\<exists>\<rhd>p)s \<longrightarrow> valid_arch_obj ao s
+            | _ \<Rightarrow> True)\<rbrace>
+  set_object p ko 
+  \<lbrace>\<lambda>_. valid_arch_objs\<rbrace>"
+  apply (simp add: valid_arch_objs_def)
+  apply (subst imp_conv_disj)+
+  apply (wp hoare_vcg_all_lift hoare_vcg_disj_lift set_object_neg_lookup set_object_neg_ko 
+            valid_arch_obj_typ2 [where Q="typ_at (a_type ko) p"] set_object_typ_at
+         | simp)+
+  apply (clarsimp simp: pred_neg_def obj_at_def)
+  apply fastforce
+  done
+
+
+lemma set_object_valid_kernel_mappings:
+  "\<lbrace>\<lambda>s. valid_kernel_mappings s
+           \<and> valid_kernel_mappings_if_pd
+                (set (arm_global_pts (arch_state s)))
+                    ko\<rbrace>
+     set_object ptr ko
+   \<lbrace>\<lambda>rv. valid_kernel_mappings\<rbrace>"
+  apply (simp add: set_object_def)
+  apply wp
+  apply (clarsimp simp: valid_kernel_mappings_def
+                 elim!: ranE split: split_if_asm)
+  apply fastforce
+  done
+
+lemma valid_vs_lookup_lift:
+  assumes lookup: "\<And>P. \<lbrace>\<lambda>s. P (vs_lookup_pages s)\<rbrace> f \<lbrace>\<lambda>_ s. P (vs_lookup_pages s)\<rbrace>"
+  assumes cap: "\<And>P. \<lbrace>\<lambda>s. P (caps_of_state s)\<rbrace> f \<lbrace>\<lambda>_ s. P (caps_of_state s)\<rbrace>"
+  assumes pts: "\<And>P. \<lbrace>\<lambda>s. P (arm_global_pts (arch_state s))\<rbrace> f \<lbrace>\<lambda>_ s. P (arm_global_pts (arch_state s))\<rbrace>"
+  shows "\<lbrace>valid_vs_lookup\<rbrace> f \<lbrace>\<lambda>_. valid_vs_lookup\<rbrace>"
+  unfolding valid_vs_lookup_def
+  apply (rule hoare_lift_Pf [where f=vs_lookup_pages])
+   apply (rule hoare_lift_Pf [where f="\<lambda>s. (caps_of_state s)"])
+    apply (rule hoare_lift_Pf [where f="\<lambda>s. arm_global_pts (arch_state s)"])
+     apply (wp lookup cap pts)
+  done
+
+
+lemma valid_table_caps_lift:
+  assumes cap: "\<And>P. \<lbrace>\<lambda>s. P (caps_of_state s)\<rbrace> f \<lbrace>\<lambda>_ s. P (caps_of_state s)\<rbrace>"
+  assumes pts: "\<And>P. \<lbrace>\<lambda>s. P (arm_global_pts (arch_state s))\<rbrace> f \<lbrace>\<lambda>_ s. P (arm_global_pts (arch_state s))\<rbrace>"
+  assumes obj: "\<And>S p. \<lbrace>obj_at (empty_table S) p\<rbrace> f \<lbrace>\<lambda>rv. obj_at (empty_table S) p\<rbrace>"
+  shows "\<lbrace>valid_table_caps\<rbrace> f \<lbrace>\<lambda>_. valid_table_caps\<rbrace>"
+  unfolding valid_table_caps_def
+   apply (rule hoare_lift_Pf [where f="\<lambda>s. (caps_of_state s)"])
+    apply (rule hoare_lift_Pf [where f="\<lambda>s. arm_global_pts (arch_state s)"])
+     apply (wp cap pts hoare_vcg_all_lift hoare_vcg_const_imp_lift obj)
+  done
+
+lemma valid_arch_caps_lift:
+  assumes lookup: "\<And>P. \<lbrace>\<lambda>s. P (vs_lookup_pages s)\<rbrace> f \<lbrace>\<lambda>_ s. P (vs_lookup_pages s)\<rbrace>"
+  assumes cap: "\<And>P. \<lbrace>\<lambda>s. P (caps_of_state s)\<rbrace> f \<lbrace>\<lambda>_ s. P (caps_of_state s)\<rbrace>"
+  assumes pts: "\<And>P. \<lbrace>\<lambda>s. P (arm_global_pts (arch_state s))\<rbrace> f \<lbrace>\<lambda>_ s. P (arm_global_pts (arch_state s))\<rbrace>"
+  assumes obj: "\<And>S p. \<lbrace>obj_at (empty_table S) p\<rbrace> f \<lbrace>\<lambda>rv. obj_at (empty_table S) p\<rbrace>"
+  shows "\<lbrace>valid_arch_caps\<rbrace> f \<lbrace>\<lambda>_. valid_arch_caps\<rbrace>"
+  unfolding valid_arch_caps_def
+  apply (rule hoare_pre)
+   apply (wp valid_vs_lookup_lift valid_table_caps_lift lookup cap pts obj)
+  apply simp
+  done
+
+lemma valid_global_objs_lift':
+  assumes pts: "\<And>P. \<lbrace>\<lambda>s. P (arm_global_pts (arch_state s))\<rbrace> f \<lbrace>\<lambda>_ s. P (arm_global_pts (arch_state s))\<rbrace>"
+  assumes pd: "\<And>P. \<lbrace>\<lambda>s. P (arm_global_pd (arch_state s))\<rbrace> f \<lbrace>\<lambda>_ s. P (arm_global_pd (arch_state s))\<rbrace>"
+  assumes obj: "\<And>p. \<lbrace>valid_ao_at p\<rbrace> f \<lbrace>\<lambda>rv. valid_ao_at p\<rbrace>"
+  assumes ko: "\<And>ako p. \<lbrace>ko_at (ArchObj ako) p\<rbrace> f \<lbrace>\<lambda>_. ko_at (ArchObj ako) p\<rbrace>"
+  assumes emp: "\<And>pd S. 
+       \<lbrace>\<lambda>s. (v \<longrightarrow> pd = arm_global_pd (arch_state s) \<and> S = set (arm_global_pts (arch_state s)) \<and> P s)
+            \<and> obj_at (empty_table S) pd s\<rbrace>
+                 f \<lbrace>\<lambda>rv. obj_at (empty_table S) pd\<rbrace>"
+  shows "\<lbrace>\<lambda>s. valid_global_objs s \<and> (v \<longrightarrow> P s)\<rbrace> f \<lbrace>\<lambda>rv. valid_global_objs\<rbrace>"
+  unfolding valid_global_objs_def
+  apply (rule hoare_pre)
+   apply (rule hoare_use_eq [where f="\<lambda>s. arm_global_pts (arch_state s)", OF pts])
+   apply (rule hoare_use_eq [where f="\<lambda>s. arm_global_pd (arch_state s)", OF pd])
+   apply (wp obj ko emp hoare_vcg_const_Ball_lift hoare_ex_wp)
+  apply clarsimp
+  done
+
+lemmas valid_global_objs_lift
+    = valid_global_objs_lift' [where v=False, simplified]
+
+lemma arch_lifts:
+  assumes arch: "\<And>P. \<lbrace>\<lambda>s. P (arch_state s)\<rbrace> f \<lbrace>\<lambda>_ s. P (arch_state s)\<rbrace>"
+  assumes aobj_at: "\<And>P P' pd. arch_obj_pred P' \<Longrightarrow>
+    \<lbrace>\<lambda>s. P (obj_at P' pd s)\<rbrace> f \<lbrace>\<lambda>r s. P (obj_at P' pd s)\<rbrace>"
+  notes arch_obj_fun_lift_expand[simp del]
+  shows
+  valid_global_pd_mappings_lift: 
+    "\<lbrace>valid_global_pd_mappings\<rbrace> f \<lbrace>\<lambda>rv. valid_global_pd_mappings\<rbrace>" and
+  valid_arch_caps_lift_weak: 
+    "(\<And>P. \<lbrace>\<lambda>s. P (caps_of_state s)\<rbrace> f \<lbrace>\<lambda>_ s. P (caps_of_state s)\<rbrace>) \<Longrightarrow> 
+      \<lbrace>valid_arch_caps\<rbrace> f \<lbrace>\<lambda>_. valid_arch_caps\<rbrace>" and
+  valid_global_objs_lift_weak:
+    "\<lbrace>valid_global_objs\<rbrace> f \<lbrace>\<lambda>rv. valid_global_objs\<rbrace>" and
+  valid_asid_map_lift:
+    "\<lbrace>valid_asid_map\<rbrace> f \<lbrace>\<lambda>rv. valid_asid_map\<rbrace>" and
+  valid_kernel_mappings_lift:
+    "\<lbrace>valid_kernel_mappings\<rbrace> f \<lbrace>\<lambda>rv. valid_kernel_mappings\<rbrace>" and
+  valid_global_pts_lift:
+    "\<lbrace>valid_global_pts\<rbrace> f \<lbrace>\<lambda>rv. valid_global_pts\<rbrace>" and
+  valid_arch_state_lift_aobj_at:
+    "\<lbrace>valid_arch_state\<rbrace> f \<lbrace>\<lambda>rv. valid_arch_state\<rbrace>"
+  apply -
+
+  subgoal
+  apply (simp add: valid_global_pd_mappings_def valid_pd_kernel_mappings_def
+              del: valid_pd_kernel_mappings_arch_def)
+  apply (rule hoare_lift_Pf[where f="arch_state", OF _ arch])
+  apply (rule_tac f="valid_pd_kernel_mappings_arch (arm_kernel_vspace x)" in hoare_lift_Pf)
+   apply (rule aobj_at; simp)
+  apply (subst valid_pd_kernel_mappings_arch_def valid_pde_kernel_mappings_def)+
+  apply (clarsimp simp add: valid_def)
+  apply (erule_tac P=P in rsubst)
+  apply (rule ext)
+  apply (clarsimp intro!: iff_allI split: arch_kernel_obj.splits pde.splits)
+  apply (safe; clarsimp simp add: valid_pt_kernel_mappings_def
+                        simp del: valid_pt_kernel_mappings_arch_def)
+     apply (erule use_valid[OF _ aobj_at[where P="\<lambda>x. x"]]; simp)+
+   by (rule classical,
+          drule use_valid[OF _ aobj_at[where P="\<lambda>x. \<not>x", OF arch_obj_pred_fun_lift_id]],
+          simp+)+
+
+  subgoal
+  apply (rule valid_arch_caps_lift[OF _ _ arch aobj_at])
+    apply (rule vs_lookup_pages_arch_obj_at_lift[OF aobj_at arch], assumption+)
+  apply (rule empty_table.arch_only)
+  done
+
+  subgoal
+  apply (rule valid_global_objs_lift)
+      apply (wp arch)
+    apply (simp add: valid_ao_at_def)
+    apply (rule hoare_vcg_ex_lift)
+    apply (rule hoare_vcg_conj_lift)
+     apply (wp aobj_at valid_arch_obj_typ | simp | rule empty_table.arch_only)+
+  done
+
+  subgoal
+  apply (simp add: valid_asid_map_def)
+  apply (rule hoare_lift_Pf[where f="arch_state", OF _ arch])
+  apply (simp add: pd_at_asid_def)
+  by (rule vs_lookup_arch_obj_at_lift[OF aobj_at arch])
+
+  subgoal
+  apply (simp add: valid_kernel_mappings_def)
+  apply (rule hoare_lift_Pf[where f="arch_state", OF _ arch])
+  apply (simp add: valid_kernel_mappings_if_pd_def ran_def
+              del: valid_kernel_mappings_if_pd_arch_def)
+  apply (rule hoare_vcg_all_lift)
+  apply (case_tac "\<exists>ao. xa = ArchObj ao")
+   apply (rule hoare_convert_imp)
+    apply clarsimp
+    apply (rule hoare_vcg_all_lift)
+    subgoal for ao a
+    by (rule aobj_at[where P=Not and P'="\<lambda>x. x = ArchObj ao", simplified obj_at_def, simplified])
+   apply clarsimp
+   apply (case_tac ao; simp add: hoare_vcg_prop)
+  apply (clarsimp simp del: valid_kernel_mappings_if_pd_arch_def)
+  apply (case_tac xa; simp add: hoare_vcg_prop)
+  done
+
+  subgoal valid_global_pts
+  apply (simp add: valid_global_pts_def)
+  apply (rule hoare_lift_Pf[where f="arch_state", OF _ arch])
+  apply (rule hoare_vcg_ball_lift)
+  apply (rule aobj_at)
+  apply clarsimp
+  done
+  
+  subgoal
+  apply (simp add: valid_arch_state_def valid_asid_table_def)
+  apply (rule hoare_lift_Pf[where f="arch_state", OF _ arch])
+  apply (wp hoare_vcg_conj_lift hoare_vcg_ball_lift valid_global_pts | (rule aobj_at, clarsimp))+
+  done
+
+  done
+
+lemma equal_kernel_mappings_lift:
+  assumes aobj_at: "\<And>P P' pd. arch_obj_pred P' \<Longrightarrow>
+                               \<lbrace>\<lambda>s. P (obj_at P' pd s)\<rbrace> f \<lbrace>\<lambda>r s. P (obj_at P' pd s)\<rbrace>"
+  shows "\<lbrace>equal_kernel_mappings\<rbrace> f \<lbrace>\<lambda>rv. equal_kernel_mappings\<rbrace>"
+  apply (simp add: equal_kernel_mappings_def)
+  apply (rule hoare_vcg_all_lift)+
+  apply (rule hoare_convert_imp)
+   apply simp
+   apply (rule hoare_convert_imp)
+    apply (wp aobj_at[OF arch_obj_pred_arch_obj_l])
+  done
+
+lemma valid_machine_state_lift:
+  assumes memory: "\<And>P. \<lbrace>\<lambda>s. P (underlying_memory (machine_state s))\<rbrace> f \<lbrace>\<lambda>_ s. P (underlying_memory (machine_state s))\<rbrace>"
+  assumes aobj_at: "\<And>P' pd. arch_obj_pred P' \<Longrightarrow> \<lbrace>obj_at P' pd\<rbrace> f \<lbrace>\<lambda>r s. obj_at P' pd s\<rbrace>"
+  shows "\<lbrace>valid_machine_state\<rbrace> f \<lbrace>\<lambda>_. valid_machine_state\<rbrace>"
+  unfolding valid_machine_state_def
+  apply (rule hoare_lift_Pf[where f="\<lambda>s. underlying_memory (machine_state s)", OF _ memory])
+  apply (rule hoare_vcg_all_lift)
+  apply (rule hoare_vcg_disj_lift[OF _ hoare_vcg_prop])
+  apply (rule in_user_frame_lift)
+  apply (wp aobj_at)
+  apply simp
+  done
+
+(*
+lemma bool_pred_exhaust: 
+  "(P = (\<lambda>x. x)) \<or> (P = (\<lambda>x. \<not>x)) \<or> (P = (\<lambda>_. True)) \<or> (P = (\<lambda>_. False))"
+  apply (cases "P True"; cases "P False")
+  apply (rule disjI2, rule disjI2, rule disjI1, rule ext)
+  defer
+  apply (rule disjI1, rule ext)
+  defer
+  apply (rule disjI2, rule disjI1, rule ext)
+  defer
+  apply (rule disjI2, rule disjI2, rule disjI2, rule ext)
+  apply (match conclusion in "P x = _" for x \<Rightarrow> \<open>cases x; fastforce\<close>)+
+  done
+*)
+
+lemma valid_ao_at_lift:
+  assumes z: "\<And>P p T. \<lbrace>\<lambda>s. P (typ_at (AArch T) p s)\<rbrace> f \<lbrace>\<lambda>rv s. P (typ_at (AArch T) p s)\<rbrace>"
+      and y: "\<And>ao. \<lbrace>\<lambda>s. ko_at (ArchObj ao) p s\<rbrace> f \<lbrace>\<lambda>rv s. ko_at (ArchObj ao) p s\<rbrace>"
+  shows      "\<lbrace>valid_ao_at p\<rbrace> f \<lbrace>\<lambda>rv. valid_ao_at p\<rbrace>"
+  unfolding valid_ao_at_def
+  by (wp hoare_vcg_ex_lift y valid_arch_obj_typ z)
+
+lemma valid_ao_at_lift_aobj_at:
+  assumes aobj_at: "\<And>P' pd. arch_obj_pred P' \<Longrightarrow> \<lbrace>obj_at P' pd\<rbrace> f \<lbrace>\<lambda>r s. obj_at P' pd s\<rbrace>"
+  shows      "\<lbrace>valid_ao_at p\<rbrace> f \<lbrace>\<lambda>rv. valid_ao_at p\<rbrace>"
+  unfolding valid_ao_at_def
+  by (wp hoare_vcg_ex_lift valid_arch_obj_typ aobj_at | clarsimp)+
+
+lemmas set_object_v_ker_map
+    = set_object_valid_kernel_mappings
+            [unfolded valid_kernel_mappings_if_pd_def]
+
+
+crunch v_ker_map[wp]: set_notification "valid_kernel_mappings"
+  (ignore: set_object wp: set_object_v_ker_map crunch_wps)
+
+
+lemma set_object_asid_map:
+  "\<lbrace>valid_asid_map and
+    obj_at (\<lambda>ko'. vs_refs ko' \<subseteq> vs_refs ko) p\<rbrace>
+  set_object p ko
+  \<lbrace>\<lambda>_. valid_asid_map\<rbrace>"
+  apply (simp add: valid_asid_map_def set_object_def)
+  apply wp
+  apply (clarsimp simp: pd_at_asid_def simp del: fun_upd_apply)
+  apply (drule bspec, blast)
+  apply clarsimp
+  apply (rule vs_lookup_stateI, assumption)
+   apply (clarsimp simp: obj_at_def)
+   apply blast
+  apply simp
+  done
+
+lemma set_object_equal_mappings:
+  "\<lbrace>\<lambda>s. equal_kernel_mappings s
+          \<and> (\<forall>pd. ko = ArchObj (PageDirectory pd)
+                \<longrightarrow> (\<forall>x pd'. ko_at (ArchObj (PageDirectory pd')) x s
+                         \<longrightarrow> (\<forall>w \<in> kernel_mapping_slots. pd w = pd' w)))\<rbrace>
+     set_object p ko
+   \<lbrace>\<lambda>rv. equal_kernel_mappings\<rbrace>"
+  apply (simp add: set_object_def, wp)
+  apply (clarsimp simp: equal_kernel_mappings_def obj_at_def
+             split del: split_if)
+  apply (simp split: split_if_asm)
+  done
+
+lemma valid_global_pd_mappings_pres:
+  "\<lbrakk> valid_global_pd_mappings s;
+     \<And>pd. ko_at (ArchObj (PageDirectory pd)) (arm_global_pd (arch_state s)) s
+            \<Longrightarrow> ko_at (ArchObj (PageDirectory pd)) (arm_global_pd (arch_state s)) s';
+     \<And>pt p. \<lbrakk> ko_at (ArchObj (PageTable pt)) p s;
+               valid_global_objs s \<Longrightarrow> p \<in> set (arm_global_pts (arch_state s)) \<rbrakk>
+            \<Longrightarrow> ko_at (ArchObj (PageTable pt)) p s';
+     arm_global_pd (arch_state s') = arm_global_pd (arch_state s);
+     arm_kernel_vspace (arch_state s') = arm_kernel_vspace (arch_state s) \<rbrakk>
+        \<Longrightarrow> valid_global_pd_mappings s'"
+  apply atomize
+  apply (clarsimp simp: valid_global_pd_mappings_def obj_at_def)
+  apply (clarsimp simp: valid_pd_kernel_mappings_def
+                 split: kernel_object.split_asm arch_kernel_obj.split_asm)
+  apply (drule_tac x=x in spec)
+  apply (clarsimp simp: valid_pde_kernel_mappings_def obj_at_def
+                        valid_pt_kernel_mappings_def pde_ref_def
+                 split: pde.split_asm)
+  apply (simp split: kernel_object.split_asm
+                     arch_kernel_obj.split_asm)
+  apply (drule spec, drule spec, drule(1) mp)
+  apply (drule mp)
+   apply (clarsimp simp: valid_global_objs_def obj_at_def empty_table_def)
+   apply (drule_tac x=x in spec)
+   apply (simp add: pde_ref_def)[1]
+  apply clarsimp
+  done
+
+lemma valid_global_pd_mappings_arch_update[simp]:
+  "arm_global_pd (f (arch_state s)) = arm_global_pd (arch_state s)
+   \<and> arm_kernel_vspace (f (arch_state s)) = arm_kernel_vspace (arch_state s)
+     \<Longrightarrow> valid_global_pd_mappings (arch_state_update f s) = valid_global_pd_mappings s"
+  by (simp add: valid_global_pd_mappings_def)
+
+lemma set_object_global_pd_mappings:
+  "\<lbrace>valid_global_pd_mappings
+            and (\<lambda>s. (page_directory_at p s \<or> page_table_at p s)
+                       \<longrightarrow> valid_global_objs s \<and> p \<notin> global_refs s)\<rbrace>
+     set_object p ko
+   \<lbrace>\<lambda>rv. valid_global_pd_mappings\<rbrace>"
+  apply (simp add: set_object_def, wp)
+  apply clarsimp
+  apply (erule valid_global_pd_mappings_pres)
+     apply (clarsimp simp: obj_at_def a_type_def global_refs_def)+
+  done
+
+
+lemma valid_table_caps_ptD:
+  "\<lbrakk> (caps_of_state s) p = Some (ArchObjectCap (arch_cap.PageTableCap p' None));
+     page_table_at p' s; valid_table_caps s \<rbrakk> \<Longrightarrow> 
+    \<exists>pt. ko_at (ArchObj (PageTable pt)) p' s \<and> valid_arch_obj (PageTable pt) s"
+  apply (clarsimp simp: valid_table_caps_def simp del: split_paired_All)
+  apply (erule allE)+
+  apply (erule (1) impE)  
+  apply (clarsimp simp add: is_pt_cap_def cap_asid_def)
+  apply (erule impE, rule refl)
+  apply (clarsimp simp: obj_at_def empty_table_def)
+  done
+
+lemma store_pde_pred_tcb_at:
+  "\<lbrace>pred_tcb_at proj P t\<rbrace> store_pde ptr val \<lbrace>\<lambda>rv. pred_tcb_at proj P t\<rbrace>"
+  apply (simp add: store_pde_def set_pd_def set_object_def
+                   get_pd_def bind_assoc)
+  apply (rule hoare_seq_ext [OF _ get_object_sp])
+  apply (case_tac x, simp_all)
+  apply (rename_tac arch_kernel_obj)
+  apply (case_tac arch_kernel_obj, simp_all)
+  apply (rule hoare_seq_ext [OF _ get_object_sp])
+  apply wp
+  apply (clarsimp simp: pred_tcb_at_def obj_at_def)
+  done
+
+lemma empty_table_lift:
+  assumes S: "\<And>P. \<lbrace>\<lambda>s. P (S s)\<rbrace> f \<lbrace>\<lambda>_ s. P (S s)\<rbrace>"
+  assumes o: "\<And>P. \<lbrace>obj_at P p and Q\<rbrace> f \<lbrace>\<lambda>_. obj_at P p\<rbrace>"
+  shows "\<lbrace>\<lambda>s. obj_at (empty_table (S s)) p s \<and> Q s\<rbrace> 
+         f \<lbrace>\<lambda>_ s. obj_at (empty_table (S s)) p s\<rbrace>"
+  apply (rule hoare_lift_Pf2 [where f="S"])
+   apply (wp o S|simp)+
+  done
+
+end
+end
