proof/invariant-abstract/X64/ArchTcbAcc_AI.thy
@@ -1,0 +1,82 @@
+(*
+ * Copyright 2014, General Dynamics C4 Systems
+ *
+ * This software may be distributed and modified according to the terms of
+ * the GNU General Public License version 2. Note that NO WARRANTY is provided.
+ * See "LICENSE_GPLv2.txt" for details.
+ *
+ * @TAG(GD_GPL)
+ *)
+
+theory ArchTcbAcc_AI
+imports "../CSpace_AI"
+begin
+context Arch begin global_naming ARM
+
+lemmas cap_master_cap_simps = 
+  cap_master_cap_def[simplified cap_master_arch_cap_def, split_simps cap.split arch_cap.split]
+
+lemma cap_master_cap_arch_eqDs:
+  "cap_master_cap cap = cap.ArchObjectCap (arch_cap.PageCap ref rghts sz mapdata)
+     \<Longrightarrow> rghts = UNIV \<and> mapdata = None
+          \<and> (\<exists>rghts mapdata. cap = cap.ArchObjectCap (arch_cap.PageCap ref rghts sz mapdata))"
+  "cap_master_cap cap = cap.ArchObjectCap arch_cap.ASIDControlCap
+     \<Longrightarrow> cap = cap.ArchObjectCap arch_cap.ASIDControlCap"
+  "cap_master_cap cap = cap.ArchObjectCap (arch_cap.ASIDPoolCap pool asid)
+     \<Longrightarrow> asid = 0 \<and> (\<exists>asid. cap = cap.ArchObjectCap (arch_cap.ASIDPoolCap pool asid))"
+  "cap_master_cap cap = cap.ArchObjectCap (arch_cap.PageTableCap ptr data)
+     \<Longrightarrow> data = None \<and> (\<exists>data. cap = cap.ArchObjectCap (arch_cap.PageTableCap ptr data))"
+  "cap_master_cap cap = cap.ArchObjectCap (arch_cap.PageDirectoryCap ptr data2)
+     \<Longrightarrow> data2 = None \<and> (\<exists>data2. cap = cap.ArchObjectCap (arch_cap.PageDirectoryCap ptr data2))"
+  by (clarsimp simp: cap_master_cap_def
+              split: cap.split_asm arch_cap.split_asm)+
+
+lemmas cap_master_cap_eqDs = 
+  cap_master_cap_eqDs1 cap_master_cap_arch_eqDs
+  cap_master_cap_eqDs1 [OF sym] cap_master_cap_arch_eqDs[OF sym]
+  
+
+lemma vm_sets_diff[simp]:
+  "vm_read_only \<noteq> vm_read_write"
+  by (simp add: vm_read_write_def vm_read_only_def)
+
+
+lemmas vm_sets_diff2[simp] = not_sym[OF vm_sets_diff]
+
+lemma cap_master_cap_tcb_cap_valid_arch:
+  "\<lbrakk> cap_master_cap c = cap_master_cap c'; is_arch_cap c \<rbrakk> \<Longrightarrow>
+  tcb_cap_valid c p s = tcb_cap_valid c' p s"
+  by (simp add: cap_master_cap_def tcb_cap_valid_def tcb_cap_cases_def
+                   valid_ipc_buffer_cap_def  is_cap_simps
+            split: option.splits cap.splits arch_cap.splits
+                   Structures_A.thread_state.splits)
+
+lemma storeWord_invs[wp]:
+  "\<lbrace>in_user_frame p and invs\<rbrace> do_machine_op (storeWord p w) \<lbrace>\<lambda>rv. invs\<rbrace>"
+proof -
+  have aligned_offset_ignore:
+    "\<And>l sz. l<4 \<Longrightarrow> p && mask 2 = 0 \<Longrightarrow>
+       p+l && ~~ mask (pageBitsForSize sz) = p && ~~ mask (pageBitsForSize sz)"
+  proof -
+    fix l sz
+    assume al: "p && mask 2 = 0"
+    assume "(l::word32) < 4" hence less: "l<2^2" by simp
+    have le: "2 \<le> pageBitsForSize sz" by (case_tac sz, simp_all)
+    show "?thesis l sz"
+      by (rule is_aligned_add_helper[simplified is_aligned_mask,
+          THEN conjunct2, THEN mask_out_first_mask_some,
+          where n=2, OF al less le])
+  qed
+
+  show ?thesis
+    apply (wp dmo_invs)
+    apply (clarsimp simp: storeWord_def invs_def valid_state_def)
+    apply (fastforce simp: valid_machine_state_def in_user_frame_def
+               assert_def simpler_modify_def fail_def bind_def return_def
+               pageBits_def aligned_offset_ignore
+             split: split_if_asm)
+    done
+qed
+
+end
+end
