proof/invariant-abstract/X64/Machine_AI.thy
@@ -1,0 +1,756 @@
+(*
+ * Copyright 2014, General Dynamics C4 Systems
+ *
+ * This software may be distributed and modified according to the terms of
+ * the GNU General Public License version 2. Note that NO WARRANTY is provided.
+ * See "LICENSE_GPLv2.txt" for details.
+ *
+ * @TAG(GD_GPL)
+ *)
+
+(* 
+Properties of machine operations.
+*)
+
+theory Machine_AI
+imports "../Bits_AI"
+begin
+
+
+definition
+  "no_irq f \<equiv> \<forall>P. \<lbrace>\<lambda>s. P (irq_masks s)\<rbrace> f \<lbrace>\<lambda>_ s. P (irq_masks s)\<rbrace>"
+
+lemma wpc_helper_no_irq:
+  "no_irq f \<Longrightarrow>  wpc_helper (P, P') (Q, Q') (no_irq f)"
+  by (simp add: wpc_helper_def)
+
+wpc_setup "\<lambda>m. no_irq m" wpc_helper_no_irq
+
+ML {*
+structure CrunchNoIrqInstance : CrunchInstance =
+struct
+  type extra = unit;
+  val name = "no_irq";
+  val has_preconds = false;
+  fun mk_term _ body _ =
+    (Syntax.parse_term @{context} "no_irq") $ body;
+  fun get_precond _ = error "crunch no_irq should not be calling get_precond";
+  fun put_precond _ _ = error "crunch no_irq should not be calling put_precond";
+  val pre_thms = [];
+  val wpc_tactic = wp_cases_tactic_weak;
+  fun parse_extra ctxt extra
+        = case extra of
+            "" => (Syntax.parse_term ctxt "%_. True", ())
+          | _ => error "no_irq does not need a precondition";
+  val magic = Syntax.parse_term @{context}
+    "\<lambda>mapp_lambda_ignore. no_irq mapp_lambda_ignore"
+end;
+
+structure CrunchNoIrq : CRUNCH = Crunch(CrunchNoIrqInstance);
+*}
+
+setup {*
+  add_crunch_instance "no_irq" (CrunchNoIrq.crunch_x, CrunchNoIrq.crunch_ignore_add_del)
+*}
+
+crunch_ignore (no_irq) (add:
+  bind return "when" get gets fail
+  assert put modify unless select
+  alternative assert_opt gets_the
+  returnOk throwError lift bindE
+  liftE whenE unlessE throw_opt
+  assertE liftM liftME sequence_x
+  zipWithM_x mapM_x sequence mapM sequenceE_x
+  mapME_x catch select_f
+  handleE' handleE handle_elseE forM forM_x
+  zipWithM ignore_failure)
+
+context Arch begin
+
+lemma det_getRegister: "det (getRegister x)"
+  by (simp add: getRegister_def)
+
+lemma det_setRegister: "det (setRegister x w)"
+  by (simp add: setRegister_def det_def modify_def get_def put_def bind_def)
+
+
+lemma det_getRestartPC: "det getRestartPC"
+  by (simp add: getRestartPC_def det_getRegister)
+  
+
+lemma det_setNextPC: "det (setNextPC p)"
+  by (simp add: setNextPC_def det_setRegister)
+
+
+lemma ef_loadWord: "empty_fail (loadWord x)"
+  by (simp add: loadWord_def)
+
+
+lemma ef_storeWord: "empty_fail (storeWord x y)"
+  by (simp add: storeWord_def)
+
+
+lemma no_fail_getRestartPC: "no_fail \<top> getRestartPC"
+  by (simp add: getRestartPC_def getRegister_def)
+
+
+lemma no_fail_loadWord [wp]: "no_fail (\<lambda>_. is_aligned p 2) (loadWord p)"
+  apply (simp add: loadWord_def is_aligned_mask [symmetric])
+  apply (rule no_fail_pre)
+   apply wp
+  apply simp
+  done
+
+
+lemma no_fail_storeWord: "no_fail (\<lambda>_. is_aligned p 2) (storeWord p w)"
+  apply (simp add: storeWord_def is_aligned_mask [symmetric])
+  apply (rule no_fail_pre)
+   apply (wp)
+  apply simp
+  done
+
+
+lemma no_fail_machine_op_lift [simp]:
+  "no_fail \<top> (machine_op_lift f)"
+  by (simp add: machine_op_lift_def)
+
+
+lemma ef_machine_op_lift [simp]:
+  "empty_fail (machine_op_lift f)"
+  by (simp add: machine_op_lift_def)
+
+
+
+lemma no_fail_setNextPC: "no_fail \<top> (setNextPC pc)"
+  by (simp add: setNextPC_def setRegister_def)
+
+
+lemma no_fail_getFAR: "no_fail \<top> getFAR"
+  by (simp add: getFAR_def)
+
+
+lemma no_fail_getDFSR: "no_fail \<top> getDFSR"
+  by (simp add: getDFSR_def)
+
+
+lemma no_fail_getIFSR: "no_fail \<top> getIFSR"
+  by (simp add: getIFSR_def)
+
+lemma no_fail_isb: "no_fail \<top> isb"
+  by (simp add: isb_def)
+
+lemma no_fail_dsb: "no_fail \<top> dsb"
+  by (simp add: dsb_def)
+
+lemma no_fail_dmb: "no_fail \<top> dmb"
+  by (simp add: dmb_def)
+
+lemma no_fail_writeTTBR0: "no_fail \<top> (writeTTBR0 w)"
+  by (simp add: writeTTBR0_def)
+
+lemma no_fail_setCurrentPD: "no_fail \<top> (setCurrentPD w)"
+  apply (simp add: setCurrentPD_def)
+  apply (rule no_fail_pre, wp no_fail_dsb no_fail_writeTTBR0 no_fail_isb, simp)
+  done
+
+lemma no_fail_cleanByVA: "no_fail \<top> (cleanByVA w p)"
+  by (simp add: cleanByVA_def)
+
+lemma no_fail_cleanByVA_PoU: "no_fail \<top> (cleanByVA_PoU w p)"
+  by (simp add: cleanByVA_PoU_def)
+
+lemma no_fail_invalidateTLB: "no_fail \<top> invalidateTLB"
+  by (simp add: invalidateTLB_def)
+
+lemma no_fail_invalidateTLB_ASID: "no_fail \<top> (invalidateTLB_ASID x)"
+  by (simp add: invalidateTLB_ASID_def)
+
+lemma no_fail_invalidateTLB_VAASID: "no_fail \<top> (invalidateTLB_VAASID x)"
+  by (simp add: invalidateTLB_VAASID_def)
+
+lemma no_fail_invalidateByVA: "no_fail \<top> (invalidateByVA w p)"
+  by (simp add: invalidateByVA_def)
+
+lemma no_fail_invalidateByVA_I: "no_fail \<top> (invalidateByVA_I w p)"
+  by (simp add: invalidateByVA_I_def)
+
+lemma no_fail_invalidate_I_PoU: "no_fail \<top> invalidate_I_PoU"
+  by (simp add: invalidate_I_PoU_def)
+
+lemma no_fail_cleanInvalByVA: "no_fail \<top> (cleanInvalByVA w p)"
+  by (simp add: cleanInvalByVA_def)
+
+lemma no_fail_branchFlush: "no_fail \<top> (branchFlush w p)"
+  by (simp add: branchFlush_def)
+
+lemma no_fail_clean_D_PoU: "no_fail \<top> clean_D_PoU"
+  by (simp add: clean_D_PoU_def)
+
+lemma no_fail_cleanInvalidate_D_PoC: "no_fail \<top> cleanInvalidate_D_PoC"
+  by (simp add: cleanInvalidate_D_PoC_def)
+
+lemma no_fail_cleanInvalidateL2Range: "no_fail \<top> (cleanInvalidateL2Range w p)"
+  by (simp add: cleanInvalidateL2Range_def)
+
+lemma no_fail_invalidateL2Range: "no_fail \<top> (invalidateL2Range w p)"
+  by (simp add: invalidateL2Range_def)
+
+lemma no_fail_cleanL2Range: "no_fail \<top> (cleanL2Range w p)"
+  by (simp add: cleanL2Range_def)
+
+lemma no_fail_initL2Cache: "no_fail \<top> initL2Cache"
+  by (simp add: initL2Cache_def)
+
+lemma no_fail_clearExMonitor: "no_fail \<top> clearExMonitor"
+  by (simp add: clearExMonitor_def)
+
+lemma no_fail_flushBTAC: "no_fail \<top> flushBTAC"
+  by (simp add: flushBTAC_def)
+
+lemma no_fail_writeContextID: "no_fail \<top> writeContextID"
+  by (simp add: writeContextID_def)
+
+lemma no_fail_setHardwareASID: "no_fail \<top> (setHardwareASID hw_asid)"
+  by (simp add: setHardwareASID_def)
+
+
+lemma no_fail_resetTimer[wp]: "no_fail \<top> resetTimer"
+  by (simp add: resetTimer_def)
+
+
+lemma loadWord_inv: "\<lbrace>P\<rbrace> loadWord x \<lbrace>\<lambda>x. P\<rbrace>"
+  apply (simp add: loadWord_def)
+  apply wp
+  apply simp
+  done
+
+
+lemma getRestartPC_inv: "\<lbrace>P\<rbrace> getRestartPC \<lbrace>\<lambda>rv. P\<rbrace>"
+  by (simp add: getRestartPC_def getRegister_def)
+
+
+lemma getDFSR_inv: "\<lbrace>P\<rbrace> getDFSR \<lbrace>\<lambda>_. P\<rbrace>"
+  by (simp add: getDFSR_def)
+
+
+lemma getFAR_inv: "\<lbrace>P\<rbrace> getFAR \<lbrace>\<lambda>_. P\<rbrace>"
+  by (simp add: getFAR_def)
+
+
+lemma getIFSR_inv: "\<lbrace>P\<rbrace> getIFSR \<lbrace>\<lambda>_. P\<rbrace>"
+  by (simp add: getIFSR_def)
+
+
+lemma no_fail_cacheRangeOp[simp, wp]:
+  assumes nf: "\<And>a b. no_fail \<top> (oper a b)"
+  shows "no_fail \<top> (cacheRangeOp oper s e p)"
+  apply (simp add: cacheRangeOp_def mapM_x_mapM)
+  apply (rule no_fail_pre)
+   apply (wp_trace no_fail_mapM nf | wpc | clarsimp)+
+  done
+
+lemma no_fail_cleanCacheRange_PoU[simp, wp]:
+  "no_fail \<top> (cleanCacheRange_PoU s e p)"
+  by (simp add: cleanCacheRange_PoU_def, wp no_fail_cleanByVA_PoU)
+
+lemma no_fail_cleanCacheRange_PoC[simp, wp]:
+  "no_fail \<top> (cleanCacheRange_PoC s e p)"
+  by (simp add: cleanCacheRange_PoC_def, wp no_fail_cleanByVA)
+
+lemma no_fail_cleanInvalidateCacheRange_RAM[simp, wp]:
+  "no_fail \<top> (cleanInvalidateCacheRange_RAM s e p)"
+  by (simp add: cleanInvalidateCacheRange_RAM_def, rule no_fail_pre, 
+      wp no_fail_dsb no_fail_cleanInvalidateL2Range no_fail_cleanInvalByVA, simp)
+
+lemma no_fail_cleanCacheRange_RAM[simp, wp]:
+  "no_fail \<top> (cleanCacheRange_RAM s e p)"
+  apply (simp add: cleanCacheRange_RAM_def)
+  apply (rule no_fail_pre, wp no_fail_dsb no_fail_cleanL2Range, simp)
+  done
+
+lemma no_fail_invalidateCacheRange_I[simp, wp]:
+  "no_fail \<top> (invalidateCacheRange_I s e p)"
+  by (simp add: invalidateCacheRange_I_def, wp no_fail_invalidateByVA_I)
+
+lemma no_fail_invalidateCacheRange_RAM[simp, wp]:
+  "no_fail \<top> (invalidateCacheRange_RAM s e p)"
+  apply (simp add: invalidateCacheRange_RAM_def lineStart_def cacheLineBits_def)
+  apply (rule no_fail_pre, wp no_fail_invalidateL2Range no_fail_invalidateByVA no_fail_dsb, simp)
+   apply (auto intro: hoare_post_taut)
+  done
+  
+lemma no_fail_branchFlushRange[simp, wp]:
+  "no_fail \<top> (branchFlushRange s e p)"
+  by (simp add: branchFlushRange_def, wp no_fail_branchFlush)
+
+lemma no_fail_cleanCaches_PoU[simp, wp]:
+  "no_fail \<top> cleanCaches_PoU"
+  by (simp add: cleanCaches_PoU_def, rule no_fail_pre, 
+      wp no_fail_dsb no_fail_clean_D_PoU no_fail_invalidate_I_PoU, simp)
+
+lemma no_fail_cleanInvalidateL1Caches[simp, wp]:
+  "no_fail \<top> cleanInvalidateL1Caches"
+  by (simp add: cleanInvalidateL1Caches_def, rule no_fail_pre, 
+      wp no_fail_dsb no_fail_cleanInvalidate_D_PoC no_fail_invalidate_I_PoU, simp)
+
+lemma no_fail_clearMemory[simp, wp]: 
+  "no_fail (\<lambda>_. is_aligned p 2) (clearMemory p b)"
+  apply (simp add: clearMemory_def mapM_x_mapM)
+  apply (rule no_fail_pre)
+   apply (wp no_fail_mapM' no_fail_storeWord no_fail_cleanCacheRange_PoU)
+  apply (clarsimp simp: upto_enum_step_def)
+  apply (erule aligned_add_aligned)
+   apply (simp add: word_size_def)
+   apply (rule is_aligned_mult_triv2 [where n = 2, simplified])
+  apply simp
+  done
+
+lemma no_fail_freeMemory[simp, wp]:
+  "no_fail (\<lambda>_. is_aligned p 2) (freeMemory p b)"
+  apply (simp add: freeMemory_def mapM_x_mapM)
+  apply (rule no_fail_pre)
+  apply (wp no_fail_mapM' no_fail_storeWord)
+  apply (clarsimp simp: upto_enum_step_def)
+  apply (erule aligned_add_aligned)
+   apply (simp add: word_size_def)
+   apply (rule is_aligned_mult_triv2 [where n = 2, simplified])
+  apply simp
+  done
+
+
+lemma no_fail_getActiveIRQ[wp]:
+  "no_fail \<top> getActiveIRQ"
+  apply (simp add: getActiveIRQ_def)
+  apply (rule no_fail_pre)
+   apply (wp non_fail_select)
+  apply simp
+  done
+
+definition "irq_state_independent P \<equiv> \<forall>f s. P s \<longrightarrow> P (irq_state_update f s)"
+
+lemma getActiveIRQ_inv [wp]:
+  "\<lbrakk>irq_state_independent P\<rbrakk> \<Longrightarrow> \<lbrace>P\<rbrace> getActiveIRQ \<lbrace>\<lambda>rv. P\<rbrace>"
+  apply (simp add: getActiveIRQ_def)
+  apply (wp alternative_wp select_wp)
+  apply (simp add: irq_state_independent_def)
+  done
+
+lemma no_fail_ackInterrupt[wp]: "no_fail \<top> (ackInterrupt irq)"
+  by (simp add: ackInterrupt_def)
+  
+
+lemma no_fail_maskInterrupt[wp]: "no_fail \<top> (maskInterrupt irq bool)"
+  by (simp add: maskInterrupt_def)
+
+
+
+lemma no_irq_use:
+  "\<lbrakk> no_irq f; (rv,s') \<in> fst (f s) \<rbrakk> \<Longrightarrow> irq_masks s' = irq_masks s"
+  apply (simp add: no_irq_def valid_def)
+  apply (erule_tac x="\<lambda>x. x = irq_masks s" in allE)
+  apply fastforce
+  done
+
+lemma machine_rest_lift_no_irq:
+  "no_irq (machine_rest_lift f)"
+  apply (clarsimp simp: no_irq_def machine_rest_lift_def split_def)
+  apply wp
+  apply simp
+  done
+
+crunch (no_irq) no_irq[wp, simp]: machine_op_lift
+
+lemma no_irq:
+  "no_irq f \<Longrightarrow> \<lbrace>\<lambda>s. P (irq_masks s)\<rbrace> f \<lbrace>\<lambda>_ s. P (irq_masks s)\<rbrace>"
+  by (simp add: no_irq_def)
+
+lemma no_irq_isb: "no_irq  isb"
+  by (simp add: isb_def)
+
+lemma no_irq_dsb: "no_irq  dsb"
+  by (simp add: dsb_def)
+
+lemma no_irq_dmb: "no_irq  dmb"
+  by (simp add: dmb_def)
+
+lemma no_irq_cleanByVA: "no_irq  (cleanByVA w p)"
+  by (simp add: cleanByVA_def)
+
+lemma no_irq_cleanByVA_PoU: "no_irq  (cleanByVA_PoU w p)"
+  by (simp add: cleanByVA_PoU_def)
+
+lemma no_irq_invalidateTLB: "no_irq  invalidateTLB"
+  by (simp add: invalidateTLB_def)
+
+lemma no_irq_invalidateTLB_ASID: "no_irq  (invalidateTLB_ASID x)"
+  by (simp add: invalidateTLB_ASID_def)
+
+lemma no_irq_invalidateTLB_VAASID: "no_irq  (invalidateTLB_VAASID x)"
+  by (simp add: invalidateTLB_VAASID_def)
+
+lemma no_irq_invalidateByVA: "no_irq  (invalidateByVA w p)"
+  by (simp add: invalidateByVA_def)
+
+lemma no_irq_invalidateByVA_I: "no_irq  (invalidateByVA_I w p)"
+  by (simp add: invalidateByVA_I_def)
+
+lemma no_irq_invalidate_I_PoU: "no_irq  invalidate_I_PoU"
+  by (simp add: invalidate_I_PoU_def)
+
+lemma no_irq_cleanInvalByVA: "no_irq  (cleanInvalByVA w p)"
+  by (simp add: cleanInvalByVA_def)
+
+lemma no_irq_branchFlush: "no_irq  (branchFlush w p)"
+  by (simp add: branchFlush_def)
+
+lemma no_irq_clean_D_PoU: "no_irq  clean_D_PoU"
+  by (simp add: clean_D_PoU_def)
+
+lemma no_irq_cleanInvalidate_D_PoC: "no_irq  cleanInvalidate_D_PoC"
+  by (simp add: cleanInvalidate_D_PoC_def)
+
+lemma no_irq_cleanInvalidateL2Range: "no_irq  (cleanInvalidateL2Range w p)"
+  by (simp add: cleanInvalidateL2Range_def)
+
+lemma no_irq_invalidateL2Range: "no_irq  (invalidateL2Range w p)"
+  by (simp add: invalidateL2Range_def)
+
+lemma no_irq_cleanL2Range: "no_irq  (cleanL2Range w p)"
+  by (simp add: cleanL2Range_def)
+
+lemma no_irq_initL2Cache: "no_irq  initL2Cache"
+  by (simp add: initL2Cache_def)
+
+lemma no_irq_flushBTAC: "no_irq  flushBTAC"
+  by (simp add: flushBTAC_def)
+
+lemma no_irq_writeContextID: "no_irq  writeContextID"
+  by (simp add: writeContextID_def)
+
+
+lemma no_irq_setHardwareASID: "no_irq (setHardwareASID hw_asid)"
+  by (simp add: setHardwareASID_def)
+
+lemma no_irq_writeTTBR0: "no_irq (writeTTBR0 pd)"
+  by (simp add: writeTTBR0_def)
+ 
+lemma no_irq_gets [simp]:
+  "no_irq (gets f)"
+  by (simp add: no_irq_def)
+
+
+lemma no_irq_getIFSR: "no_irq getIFSR"
+  by (simp add: getIFSR_def)
+
+
+lemma no_irq_getDFSR: "no_irq getDFSR"
+  by (simp add: getDFSR_def)
+
+
+lemma no_irq_getFAR: "no_irq getFAR"
+  by (simp add: getFAR_def)
+
+
+lemma no_irq_resetTimer: "no_irq resetTimer"
+  by (simp add: resetTimer_def)
+
+
+lemma no_irq_debugPrint: "no_irq (debugPrint $ xs)"
+  by (simp add: no_irq_def)
+
+context notes no_irq[wp] begin
+
+lemma no_irq_ackInterrupt: "no_irq (ackInterrupt irq)"
+  by (wp | clarsimp simp: no_irq_def ackInterrupt_def)+
+
+lemma no_irq_loadWord: "no_irq (loadWord x)"
+  apply (clarsimp simp: no_irq_def)
+  apply (rule loadWord_inv)
+  done
+
+
+lemma no_irq_getActiveIRQ: "no_irq getActiveIRQ"
+  apply (clarsimp simp: no_irq_def)
+  apply (rule getActiveIRQ_inv)
+  apply (simp add: irq_state_independent_def)
+  done
+
+
+lemma no_irq_mapM:
+  "(\<And>x. x \<in> set xs \<Longrightarrow> no_irq (f x)) \<Longrightarrow> no_irq (mapM f xs)"
+  apply (subst no_irq_def)
+  apply clarify
+  apply (rule mapM_wp)
+   prefer 2
+   apply (rule order_refl)
+  apply wp
+  apply simp
+  done
+
+
+lemma no_irq_mapM_x:
+  "(\<And>x. x \<in> set xs \<Longrightarrow> no_irq (f x)) \<Longrightarrow> no_irq (mapM_x f xs)"
+  apply (subst no_irq_def)
+  apply clarify
+  apply (rule mapM_x_wp)
+   prefer 2
+   apply (rule order_refl)
+  apply wp
+  apply simp
+  done
+  
+
+lemma no_irq_swp:
+  "no_irq (f y x) \<Longrightarrow> no_irq (swp f x y)"
+  by (simp add: swp_def)
+
+
+lemma no_irq_seq [wp]:
+  "\<lbrakk> no_irq f; \<And>x. no_irq (g x) \<rbrakk> \<Longrightarrow> no_irq (f >>= g)"
+  apply (subst no_irq_def)
+  apply clarsimp
+  apply (rule hoare_seq_ext)
+  apply (wp|simp)+
+  done
+
+lemma no_irq_return [simp, wp]: "no_irq (return v)"
+  unfolding no_irq_def return_def
+  by (rule allI, simp add: valid_def)
+
+
+lemma no_irq_fail [simp, wp]: "no_irq fail"
+  unfolding no_irq_def fail_def
+  by (rule allI, simp add: valid_def)
+
+
+
+lemma no_irq_assert [simp, wp]: "no_irq (assert P)"
+  unfolding assert_def by simp
+
+
+lemma no_irq_modify:
+  "(\<And>s. irq_masks (f s) = irq_masks s) \<Longrightarrow> no_irq (modify f)"
+  unfolding modify_def no_irq_def
+  apply (rule allI, simp add: valid_def put_def get_def)
+  apply (clarsimp simp: in_monad)
+  done
+
+lemma no_irq_setCurrentPD: "no_irq (setCurrentPD pd)"
+  apply (clarsimp simp: setCurrentPD_def)
+  apply (wp no_irq_dsb no_irq_writeTTBR0 no_irq_isb)
+  done
+
+lemma no_irq_clearExMonitor: "no_irq clearExMonitor"
+  apply (simp add: clearExMonitor_def)
+  apply (wp no_irq_modify)
+  apply simp
+  done
+
+
+lemma no_irq_storeWord: "no_irq (storeWord w p)"
+  apply (simp add: storeWord_def)    
+  apply (wp no_irq_modify)
+  apply simp
+  done
+
+lemma no_irq_cacheRangeOp[simp, wp]:
+  assumes nf: "\<And>a b. no_irq (oper a b)"
+  shows "no_irq (cacheRangeOp oper s e p)"
+  apply (simp add: cacheRangeOp_def)
+   apply (wp_trace no_irq_mapM_x nf | wpc | clarsimp)+
+  done
+
+lemma no_irq_cleanCacheRange_PoU[simp, wp]:
+  "no_irq (cleanCacheRange_PoU s e p)"
+  by (simp add: cleanCacheRange_PoU_def, wp no_irq_cleanByVA_PoU)
+
+lemma no_irq_cleanCacheRange_PoC[simp, wp]:
+  "no_irq (cleanCacheRange_PoC s e p)"
+  by (simp add: cleanCacheRange_PoC_def, wp no_irq_cleanByVA)
+
+lemma no_irq_cleanInvalidateCacheRange_RAM[simp, wp]:
+  "no_irq (cleanInvalidateCacheRange_RAM s e p)"
+  by (simp add: cleanInvalidateCacheRange_RAM_def, 
+      wp no_irq_dsb no_irq_cleanInvalidateL2Range no_irq_cleanInvalByVA)
+
+lemma no_irq_cleanCacheRange_RAM[simp, wp]:
+  "no_irq (cleanCacheRange_RAM s e p)"
+  apply (simp add: cleanCacheRange_RAM_def)
+  apply (wp no_irq_dsb no_irq_cleanL2Range)
+  done
+
+lemma no_irq_invalidateCacheRange_I[simp, wp]:
+  "no_irq (invalidateCacheRange_I s e p)"
+  by (simp add: invalidateCacheRange_I_def, wp no_irq_invalidateByVA_I)
+
+lemma no_irq_when:
+  "\<lbrakk>P \<Longrightarrow> no_irq f\<rbrakk> \<Longrightarrow> no_irq (when P f)"
+  by (simp add: when_def)
+
+lemma no_irq_invalidateCacheRange_RAM[simp, wp]:
+  "no_irq (invalidateCacheRange_RAM s e p)"
+  apply (simp add: invalidateCacheRange_RAM_def lineStart_def cacheLineBits_def)
+  apply (wp no_irq_invalidateL2Range no_irq_invalidateByVA no_irq_dsb no_irq_when)
+  done
+  
+lemma no_irq_branchFlushRange[simp, wp]:
+  "no_irq (branchFlushRange s e p)"
+  by (simp add: branchFlushRange_def, wp no_irq_branchFlush)
+
+lemma no_irq_cleanCaches_PoU[simp, wp]:
+  "no_irq cleanCaches_PoU"
+  by (simp add: cleanCaches_PoU_def,
+      wp no_irq_dsb no_irq_clean_D_PoU no_irq_invalidate_I_PoU)
+
+lemma no_irq_cleanInvalidateL1Caches[simp, wp]:
+  "no_irq cleanInvalidateL1Caches"
+  by (simp add: cleanInvalidateL1Caches_def, 
+      wp no_irq_dsb no_irq_cleanInvalidate_D_PoC no_irq_invalidate_I_PoU)
+
+
+lemma no_irq_clearMemory: "no_irq (clearMemory a b)"
+  apply (simp add: clearMemory_def)
+  apply (wp no_irq_mapM_x no_irq_storeWord no_irq_cleanCacheRange_PoU)
+  done
+
+lemma getActiveIRQ_le_maxIRQ':
+  "\<lbrace>\<lambda>s. \<forall>irq > maxIRQ. irq_masks s irq\<rbrace> getActiveIRQ \<lbrace>\<lambda>rv s. \<forall>x. rv = Some x \<longrightarrow> x \<le> maxIRQ\<rbrace>"
+  apply (simp add: getActiveIRQ_def)
+  apply (wp alternative_wp select_wp)
+  apply clarsimp
+  apply (rule ccontr)
+  apply (simp add: linorder_not_le)
+  done
+
+(* FIXME: follows already from getActiveIRQ_le_maxIRQ *)
+lemma getActiveIRQ_neq_Some0xFF':
+  "\<lbrace>\<top>\<rbrace> getActiveIRQ \<lbrace>\<lambda>rv s. rv \<noteq> Some 0x3FF\<rbrace>"
+  apply (simp add: getActiveIRQ_def)
+  apply (wp alternative_wp select_wp)
+  apply simp
+  done
+
+lemma empty_fail_isb: "empty_fail  isb"
+  by (simp add: isb_def)
+
+lemma empty_fail_dsb: "empty_fail  dsb"
+  by (simp add: dsb_def)
+
+lemma empty_fail_dmb: "empty_fail  dmb"
+  by (simp add: dmb_def)
+
+lemma empty_fail_cleanByVA: "empty_fail  (cleanByVA w p)"
+  by (simp add: cleanByVA_def)
+
+lemma empty_fail_cleanByVA_PoU: "empty_fail  (cleanByVA_PoU w p)"
+  by (simp add: cleanByVA_PoU_def)
+
+lemma empty_fail_invalidateTLB: "empty_fail  invalidateTLB"
+  by (simp add: invalidateTLB_def)
+
+lemma empty_fail_invalidateTLB_ASID: "empty_fail  (invalidateTLB_ASID x)"
+  by (simp add: invalidateTLB_ASID_def)
+
+lemma empty_fail_invalidateTLB_VAASID: "empty_fail  (invalidateTLB_VAASID x)"
+  by (simp add: invalidateTLB_VAASID_def)
+
+lemma empty_fail_invalidateByVA: "empty_fail  (invalidateByVA w p)"
+  by (simp add: invalidateByVA_def)
+
+lemma empty_fail_invalidateByVA_I: "empty_fail  (invalidateByVA_I w p)"
+  by (simp add: invalidateByVA_I_def)
+
+lemma empty_fail_invalidate_I_PoU: "empty_fail  invalidate_I_PoU"
+  by (simp add: invalidate_I_PoU_def)
+
+lemma empty_fail_cleanInvalByVA: "empty_fail  (cleanInvalByVA w p)"
+  by (simp add: cleanInvalByVA_def)
+
+lemma empty_fail_branchFlush: "empty_fail  (branchFlush w p)"
+  by (simp add: branchFlush_def)
+
+lemma empty_fail_clean_D_PoU: "empty_fail  clean_D_PoU"
+  by (simp add: clean_D_PoU_def)
+
+lemma empty_fail_cleanInvalidate_D_PoC: "empty_fail  cleanInvalidate_D_PoC"
+  by (simp add: cleanInvalidate_D_PoC_def)
+
+lemma empty_fail_cleanInvalidateL2Range: "empty_fail  (cleanInvalidateL2Range w p)"
+  by (simp add: cleanInvalidateL2Range_def)
+
+lemma empty_fail_invalidateL2Range: "empty_fail  (invalidateL2Range w p)"
+  by (simp add: invalidateL2Range_def)
+
+lemma empty_fail_cleanL2Range: "empty_fail  (cleanL2Range w p)"
+  by (simp add: cleanL2Range_def)
+
+lemma empty_fail_initL2Cache: "empty_fail  initL2Cache"
+  by (simp add: initL2Cache_def)
+
+lemma empty_fail_clearExMonitor: "empty_fail  clearExMonitor"
+  by (simp add: clearExMonitor_def)
+
+lemma empty_fail_flushBTAC: "empty_fail  flushBTAC"
+  by (simp add: flushBTAC_def)
+
+lemma empty_fail_writeContextID: "empty_fail  writeContextID"
+  by (simp add: writeContextID_def)
+
+
+
+lemma empty_fail_cacheRangeOp [simp, intro!]:
+  assumes ef: "\<And>a b. empty_fail (oper a b)"
+  shows "empty_fail (cacheRangeOp oper s e p)"
+  apply (simp add: cacheRangeOp_def mapM_x_mapM lineStart_def cacheLineBits_def cacheLine_def ef)
+  apply (rule empty_fail_bind)
+   apply (rule empty_fail_mapM)
+   apply (auto intro: ef)
+  done
+
+
+lemma empty_fail_cleanCacheRange_PoU[simp, intro!]:
+  "empty_fail (cleanCacheRange_PoU s e p)"
+  by (simp add: cleanCacheRange_PoU_def empty_fail_cleanByVA_PoU)
+
+lemma empty_fail_cleanCacheRange_PoC[simp, intro!]:
+  "empty_fail (cleanCacheRange_PoC s e p)"
+  by (simp add: cleanCacheRange_PoC_def empty_fail_cleanByVA)
+
+lemma empty_fail_cleanInvalidateCacheRange_RAM[simp, intro!]:
+  "empty_fail (cleanInvalidateCacheRange_RAM s e p)"
+  by (simp add: cleanInvalidateCacheRange_RAM_def empty_fail_dsb empty_fail_cleanInvalidateL2Range empty_fail_cleanInvalByVA)
+
+lemma empty_fail_cleanCacheRange_RAM[simp, intro!]:
+  "empty_fail (cleanCacheRange_RAM s e p)"
+  by (simp add: cleanCacheRange_RAM_def empty_fail_dsb empty_fail_cleanL2Range)
+
+lemma empty_fail_invalidateCacheRange_I[simp, intro!]:
+  "empty_fail (invalidateCacheRange_I s e p)"
+  by (simp add: invalidateCacheRange_I_def empty_fail_invalidateByVA_I)
+
+lemma empty_fail_invalidateCacheRange_RAM[simp, intro!]:
+  "empty_fail (invalidateCacheRange_RAM s e p)"
+  by (simp add: invalidateCacheRange_RAM_def lineStart_def cacheLineBits_def 
+                   empty_fail_invalidateL2Range empty_fail_invalidateByVA empty_fail_dsb)
+  
+lemma empty_fail_branchFlushRange[simp, intro!]:
+  "empty_fail (branchFlushRange s e p)"
+  by (simp add: branchFlushRange_def empty_fail_branchFlush)
+
+lemma empty_fail_cleanCaches_PoU[simp, intro!]:
+  "empty_fail cleanCaches_PoU"
+  by (simp add: cleanCaches_PoU_def empty_fail_dsb empty_fail_clean_D_PoU empty_fail_invalidate_I_PoU)
+
+lemma empty_fail_cleanInvalidateL1Caches[simp, intro!]:
+  "empty_fail cleanInvalidateL1Caches"
+  by (simp add: cleanInvalidateL1Caches_def empty_fail_dsb empty_fail_cleanInvalidate_D_PoC 
+                empty_fail_invalidate_I_PoU)
+
+lemma empty_fail_clearMemory [simp, intro!]:
+  "\<And>a b. empty_fail (clearMemory a b)"
+  by (simp add: clearMemory_def mapM_x_mapM ef_storeWord)
+
+end
+end
+
+end
